examples/accidentes-aereos-main.dfy
@@ -1,0 +1,25 @@
+include "../src/linear/adt/Stack.dfy"
+include "../examples/accidentes-aereos.dfy"
+
+// method {:extern} Read() returns (x: int)
+// method {:extern} ScanInt() returns (x: int)
+// method {:extern} ScanString() returns (s: string)
+
+method {:verify false} Main()
+{
+  var v := new nat[6];
+  v[0] := 50;
+  v[1] := 80;
+  v[2] := 30;
+  v[3] := 10;
+  v[4] := 60;
+  v[5] := 5;
+  var st := new Stack1();
+  var r := FindSummits(v, st);
+  var i := 0;
+  while i < r.Length
+  {
+    print r[i], " ";
+    i := i + 1;
+  }
+}
